More spec integration of Blake2

specs/Spec.Hash.Definitions.fst
@@ -34,6 +34,8 @@ type hash_alg =
   | SHA2_512
   | SHA1
   | MD5
+  | Blake2S
+  | Blake2B
 
 // BB. Remove when renamed.
 let algorithm = hash_alg
@@ -42,8 +44,16 @@ let is_sha2 = function
   | SHA2_224 | SHA2_256 | SHA2_384 | SHA2_512 -> true
   | _ -> false
 
-let sha2_alg = a:hash_alg { is_sha2 a }
+let is_blake = function
+  | Blake2S | Blake2B -> true
+  | _ -> false
 
+let sha2_alg = a:hash_alg { is_sha2 a }
+let blake_alg = a:hash_alg { is_blake a }
+
+let to_blake_alg (a:blake_alg) = match a with
+  | Blake2S -> Spec.Blake2.Blake2S
+  | Blake2B -> Spec.Blake2.Blake2B
 
 (** Maximum input data length. *)
 
@@ -55,6 +65,8 @@ let max_input_length: hash_alg -> Tot nat = function
   | MD5 | SHA1
   | SHA2_224 | SHA2_256 -> pow2 61 - 1
   | SHA2_384 | SHA2_512 -> pow2 125 - 1
+  | Blake2S -> pow2 64 - 1
+  | Blake2B -> pow2 128 - 1
 
 // BB. Removed once renamed...
 let max_input = max_input_length
@@ -65,6 +77,8 @@ let len_int_type: hash_alg -> inttype = function
   | MD5 | SHA1
   | SHA2_224 | SHA2_256 -> U64
   | SHA2_384 | SHA2_512 -> U128
+  | Blake2S -> U64
+  | Blake2B -> U128
 
 inline_for_extraction
 let nat_to_len (a:hash_alg) (n:nat{n <= maxint (len_int_type a)}) =
@@ -76,12 +90,16 @@ let len_t: hash_alg -> Type = function
   | MD5 | SHA1
   | SHA2_224 | SHA2_256 -> pub_uint64
   | SHA2_384 | SHA2_512 -> pub_uint128
+  | Blake2S -> pub_uint64
+  | Blake2B -> pub_uint128
 
 val len_v: a:hash_alg -> len_t a -> nat
 let len_v = function
   | MD5 | SHA1
   | SHA2_224 | SHA2_256 -> uint_v #U64 #PUB
   | SHA2_384 | SHA2_512 -> uint_v #U128 #PUB
+  | Blake2S -> uint_v #U64 #PUB
+  | Blake2B -> uint_v #U128 #PUB
 
 (* Number of bytes occupied by a len_t, i.e. the size of the encoded length in
    the padding. *)
@@ -89,12 +107,16 @@ let len_length: hash_alg -> Tot nat = function
   | MD5 | SHA1
   | SHA2_224 | SHA2_256 -> 8
   | SHA2_384 | SHA2_512 -> 16
+  | Blake2S -> 8
+  | Blake2B -> 16
 
 (* Same thing, as a machine integer *)
 inline_for_extraction
 let len_len: a:hash_alg -> Tot (n:size_t{v n = len_length a}) = function
   | MD5 | SHA1 | SHA2_224 | SHA2_256 -> 8ul
   | SHA2_384 | SHA2_512 -> 16ul
+  | Blake2S -> 8ul
+  | Blake2B -> 16ul
 
 (** Working state of the algorithms. *)
 
@@ -104,16 +126,24 @@ let word_t: hash_alg -> Tot inttype = function
   | MD5 | SHA1
   | SHA2_224 | SHA2_256 -> U32
   | SHA2_384 | SHA2_512 -> U64
+  | Blake2S -> U32
+  | Blake2B -> U64
+
+inline_for_extraction
+let row (a:blake_alg) = lseq (uint_t (word_t a) SEC) 4
 
 inline_for_extraction
 let word (a: hash_alg) = match a with
   | MD5 | SHA1 | SHA2_224 | SHA2_256 | SHA2_384 | SHA2_512 -> uint_t (word_t a) SEC
+  | Blake2S | Blake2B -> row a
 
 (* In bytes *)
 let word_length: hash_alg -> Tot nat = function
   | MD5 | SHA1
   | SHA2_224 | SHA2_256 -> 4
   | SHA2_384 | SHA2_512 -> 8
+  | Blake2S -> 4
+  | Blake2B -> 8
 
 (* Number of words for a block size *)
 noextract
@@ -135,11 +165,18 @@ let state_word_length a =
   match a with
   | MD5 -> 4
   | SHA1 -> 5
+  | Blake2S | Blake2B -> 4
   | _ -> 8
 
 inline_for_extraction noextract
 let extra_state a = match a with
   | MD5 | SHA1 | SHA2_224 | SHA2_256 | SHA2_384 | SHA2_512 -> unit
+  // Directly storing the length instead of the number of blocks to avoid
+  // nonlinear operations in the spec
+  // We use uints to avoid reasoning about max bounds.
+  // In practice, we never have overflows because of restrictions on length of buffers
+  | Blake2S -> uint_t U64 SEC
+  | Blake2B -> uint_t U128 SEC
 
 (* The working state *)
 inline_for_extraction noextract
@@ -156,6 +193,7 @@ let hash_word_length: hash_alg -> Tot nat = function
   | SHA2_256 -> 8
   | SHA2_384 -> 6
   | SHA2_512 -> 8
+  | Blake2S | Blake2B -> 8
 
 (* Define the final hash length in bytes *)
 // BB. Needs to be renamed
@@ -185,11 +223,13 @@ let bytes_of_words: a:hash_alg -> Tot (#len:size_nat{FStar.Mul.(len * word_lengt
   | MD5 -> Lib.ByteSequence.uints_to_bytes_le #U32 #SEC
   | SHA1 | SHA2_224 | SHA2_256 -> Lib.ByteSequence.uints_to_bytes_be #U32 #SEC
   | SHA2_384 | SHA2_512 -> Lib.ByteSequence.uints_to_bytes_be #U64 #SEC
+  | Blake2S | Blake2B -> admit()
 
 let words_of_bytes: a:hash_alg -> Tot (#len:size_nat{FStar.Mul.(len * word_length a) <= max_size_t} -> b:lbytes FStar.Mul.(word_length a * len) -> Tot (lseq (word a) len)) = function
   | MD5 -> Lib.ByteSequence.uints_from_bytes_le #U32 #SEC
   | SHA1 | SHA2_224 | SHA2_256 -> Lib.ByteSequence.uints_from_bytes_be #U32 #SEC
   | SHA2_384 | SHA2_512 -> Lib.ByteSequence.uints_from_bytes_be #U64 #SEC
+  | Blake2S | Blake2B -> admit()
 
 (** The data format taken and returned by the hash specifications. *)
 
