specs/Spec.Agile.Hash.fst
@@ -4,6 +4,8 @@ module S = FStar.Seq
 
 open Spec.Hash.Definitions
 open Spec.Hash.PadFinish
+open FStar.Mul
+open Lib.IntTypes
 
 let init a =
   match a with
@@ -13,6 +15,8 @@ let init a =
       Spec.MD5.init
   | SHA1 ->
       Spec.SHA1.init
+  | Blake2S -> Spec.Blake2.blake2_init Spec.Blake2.Blake2S 0 Seq.empty 32, u64 0
+  | Blake2B -> Spec.Blake2.blake2_init Spec.Blake2.Blake2B 0 Seq.empty 64, u128 0
 
 let update a =
   match a with
@@ -22,16 +26,28 @@ let update a =
       Spec.MD5.update
   | SHA1 ->
       Spec.SHA1.update
+  | Blake2S -> fun h l ->
+      let blake_state, totlen = h in
+      (Spec.Blake2.blake2_update_block Spec.Blake2.Blake2S false (v #U64 #SEC totlen) l blake_state,
+      // We should never have overflows given the restriction on buffer lengths, so
+      // this should be equivalent to a nat addition
+       totlen +. u64 (size_block a))
+  | Blake2B -> fun h l ->
+      let blake_state, totlen = h in
+      (Spec.Blake2.blake2_update_block Spec.Blake2.Blake2B false (v #U128 #SEC totlen) l blake_state,
+      // We should never have overflows given the restriction on buffer lengths, so
+      // this should be equivalent to a nat addition
+       totlen +. u128 (size_block a))
+
 
 (* A helper that deals with the modulo proof obligation to make things go smoothly. *)
 let split_block (a: hash_alg)
   (blocks: bytes_blocks a)
   (n: nat{n <= S.length blocks / block_length a}):
-  Tot (p:(Spec.Hash.Definitions.bytes_blocks a * Spec.Hash.Definitions.bytes_blocks a)
-         {fst p == fst (Seq.split blocks (FStar.Mul.(n * block_length a))) /\
-	  snd p == snd (Seq.split blocks (FStar.Mul.(n * block_length a)))})
-=
-  let block, rem = S.split blocks FStar.Mul.(n * block_length a) in
+  Tot (p:(Spec.Hash.Definitions.bytes_blocks a & Spec.Hash.Definitions.bytes_blocks a)
+         {fst p == fst (Seq.split blocks (n * block_length a)) /\
+	  snd p == snd (Seq.split blocks (n * block_length a))})
+= let block, rem = S.split blocks (n * block_length a) in
   assert (S.length rem = S.length blocks - S.length block);
   Math.Lemmas.modulo_distributivity (S.length rem) (S.length block) (block_length a);
   assert (S.length rem % block_length a = 0);
